out/InductNatExample.v
@@ -6,169 +6,211 @@ Inductive Natural: Set := ZeroN: Natural | Suc: (Natural -> Natural).
 Load IntNatExample. 
 Definition one := Suc ZeroN. 
 Definition two := Suc one. 
+Definition toInt_unrefined (n: { n : Natural | True }): { v : BinNums.Z | v>=0 }. 
+Proof.
+  destruct n as [n np ]. 
+  induction n as [| n IHn ]. 
+    { now unshelve refine (injectionCast BinNums.Z (fun v: BinNums.Z => v>=0) (0) _). }
+    { now unshelve refine (injectionCast BinNums.Z (fun v: BinNums.Z => v>=0) (1+(` (IHn))) _). }
+Defined.
+
+Definition toInt (n: { n : Natural | True }): { v : BinNums.Z | (` (toInt_unrefined n))=v } .
+Proof.
+  destruct n as [n np ]. 
+  exact (exist (` (toInt_unrefined (injectionCast Natural (fun n: Natural => True) (n) _))) eq_refl). 
+Defined.
+
 Definition add_unrefined (m: { m : Natural | True }) (n: { n : Natural | True }): { VV : Natural | True }. 
 Proof.
   destruct m as [m mp ].  destruct n as [n np ]. 
-  induction m as [| m IHm ]. now 
- unshelve refine (injectionCast Natural (fun VV: Natural => True) (fun VV: Natural => I) (n)). now 
- unshelve refine (injectionCast Natural (fun VV: Natural => True) (fun VV: Natural => I) (Suc (` (IHm)))).
+  induction m as [| m IHm ]. 
+    { now unshelve refine (injectionCast Natural (fun VV: Natural => True) (n) _). }
+    { now unshelve refine (injectionCast Natural (fun VV: Natural => True) (Suc (` (IHm))) _). }
 Defined.
 
 Definition add (m: { m : Natural | True }) (n: { n : Natural | True }): { VV : Natural | (` (add_unrefined m n))=VV } .
 Proof.
   destruct m as [m mp ].  destruct n as [n np ]. 
-  exact (exist (` (add_unrefined (injectionCast Natural (fun m: Natural => True) (fun m: Natural => I) (m)) (injectionCast Natural (fun n: Natural => True) (fun n: Natural => I) (n)))) eq_refl). 
+  exact (exist (` (add_unrefined (injectionCast Natural (fun m: Natural => True) (m) _) (injectionCast Natural (fun n: Natural => True) (n) _))) eq_refl). 
 Defined.
 
 Definition mult_unrefined (m: { m : Natural | True }) (n: { n : Natural | True }): { VV : Natural | True }. 
 Proof.
   destruct m as [m mp ].  destruct n as [n np ]. 
-  induction m as [| m IHm ]. now 
- unshelve refine (injectionCast Natural (fun VV: Natural => True) (fun VV: Natural => I) (ZeroN)). now 
- unshelve refine (subsumptionCast Natural (fun VV: Natural => (` (add_unrefined (injectionCast Natural (fun n: Natural => True) (fun n: Natural => I) (n)) IHm))=VV) (fun VV: Natural => True) _ (add (injectionCast Natural (fun m: Natural => True) (fun m: Natural => I) (n)) IHm)).
+  induction m as [| m IHm ]. 
+    { now unshelve refine (injectionCast Natural (fun VV: Natural => True) (ZeroN) _). }
+    { now unshelve refine (subsumptionCast Natural (fun VV: Natural => (` (add_unrefined (injectionCast Natural (fun n: Natural => True) (n) _) IHm))=VV) (fun VV: Natural => True) _ (add (injectionCast Natural (fun m: Natural => True) (n) _) IHm)). }
 Defined.
 
 Definition mult (m: { m : Natural | True }) (n: { n : Natural | True }): { VV : Natural | (` (mult_unrefined m n))=VV } .
 Proof.
   destruct m as [m mp ].  destruct n as [n np ]. 
-  exact (exist (` (mult_unrefined (injectionCast Natural (fun m: Natural => True) (fun m: Natural => I) (m)) (injectionCast Natural (fun n: Natural => True) (fun n: Natural => I) (n)))) eq_refl). 
+  exact (exist (` (mult_unrefined (injectionCast Natural (fun m: Natural => True) (m) _) (injectionCast Natural (fun n: Natural => True) (n) _))) eq_refl). 
 Defined.
 
 Definition add_zero_l_spec: Prop. 
-Proof. now unshelve refine (forall (n:{n: Natural| True}), (` (add (injectionCast Natural (fun m: Natural => True) (fun m: Natural => I) (ZeroN)) n))=(` (n))).
+Proof. now unshelve refine (forall (n:{n: Natural| True}), (` (add (injectionCast Natural (fun m: Natural => True) (ZeroN) _) n))=(` (n))). .
 Defined.
 Theorem add_zero_l: add_zero_l_spec.
 Proof.
   intros n. destruct n as [n np ]. 
-  induction n as [| n IHn ]. now smt_trivial. smt_app IHn.
+  induction n as [| n IHn ]. 
+    { now smt_trivial. }
+    { smt_app IHn. }
 Qed.
 
 Definition add_suc_l_spec: Prop. 
-Proof. now unshelve refine (forall (m:{m: Natural| True}) (n:{n: Natural| True}), Suc (` (add m n))=(` (add (injectionCast Natural (fun m: Natural => True) (fun m: Natural => I) (Suc (` (m)))) n))).
+Proof. now unshelve refine (forall (m:{m: Natural| True}) (n:{n: Natural| True}), Suc (` (add m n))=(` (add (injectionCast Natural (fun m: Natural => True) (Suc (` (m))) _) n))). .
 Defined.
 Theorem add_suc_l: add_suc_l_spec.
 Proof.
   intros m. intros n. destruct m as [m mp ].  destruct n as [n np ]. 
-  induction m as [| m IHm ]. now smt_trivial. smt_app IHm.
+  induction m as [| m IHm ]. 
+    { now smt_trivial. }
+    { smt_app IHm. }
 Qed.
 
 Definition add_zero_r_spec: Prop. 
-Proof. now unshelve refine (forall (n:{n: Natural| True}), (` (add n (injectionCast Natural (fun n: Natural => True) (fun n: Natural => I) (ZeroN))))=(` (n))).
+Proof. now unshelve refine (forall (n:{n: Natural| True}), (` (add n (injectionCast Natural (fun n: Natural => True) (ZeroN) _)))=(` (n))). .
 Defined.
 Theorem add_zero_r: add_zero_r_spec.
 Proof.
   intros n. destruct n as [n np ]. 
-  induction n as [| n IHn ]. now smt_trivial. smt_app IHn.
+  induction n as [| n IHn ]. 
+    { now smt_trivial. }
+    { smt_app IHn. }
 Qed.
 
 Definition mult_one_l_spec: Prop. 
-Proof. now unshelve refine (forall (n:{n: Natural| True}), (` (mult (injectionCast Natural (fun m: Natural => True) (fun m: Natural => I) (one)) n))=(` (n))).
+Proof. now unshelve refine (forall (n:{n: Natural| True}), (` (mult (injectionCast Natural (fun m: Natural => True) (one) _) n))=(` (n))). .
 Defined.
 Theorem mult_one_l: mult_one_l_spec.
 Proof.
   intros n. destruct n as [n np ]. 
-  smt_app (add_zero_r (injectionCast Natural (fun n: Natural => True) (fun n: Natural => I) (n))).
+  
+    { smt_app (add_zero_r (injectionCast Natural (fun n: Natural => True) (n) _)). }
 Qed.
 
 Definition add_suc_r_spec: Prop. 
-Proof. now unshelve refine (forall (m:{m: Natural| True}) (n:{n: Natural| True}), Suc (` (add m n))=(` (add m (injectionCast Natural (fun n: Natural => True) (fun n: Natural => I) (Suc (` (n))))))).
+Proof. now unshelve refine (forall (m:{m: Natural| True}) (n:{n: Natural| True}), Suc (` (add m n))=(` (add m (injectionCast Natural (fun n: Natural => True) (Suc (` (n))) _)))). .
 Defined.
 Theorem add_suc_r: add_suc_r_spec.
 Proof.
   intros m. intros n. destruct m as [m mp ].  destruct n as [n np ]. 
-  induction m as [| m IHm ]. now smt_trivial. smt_app IHm.
+  induction m as [| m IHm ]. 
+    { now smt_trivial. }
+    { smt_app IHm. }
 Qed.
 
 Definition add_comm_spec: Prop. 
-Proof. now unshelve refine (forall (m:{m: Natural| True}) (n:{n: Natural| True}), (` (add m n))=(` (add n m))).
+Proof. now unshelve refine (forall (m:{m: Natural| True}) (n:{n: Natural| True}), (` (add m n))=(` (add n m))). .
 Defined.
 Theorem add_comm: add_comm_spec.
 Proof.
   intros m. intros n. destruct m as [m mp ].  destruct n as [n np ]. 
-  induction m as [| m IHm ]. smt_app (add_zero_r (injectionCast Natural (fun n: Natural => True) (fun n: Natural => I) (n))). smt_app IHm. smt_app (add_suc_r (injectionCast Natural (fun m: Natural => True) (fun m: Natural => I) (n)) (injectionCast Natural (fun n: Natural => True) (fun n: Natural => I) (m))).
+  induction m as [| m IHm ]. 
+    { smt_app (add_zero_r (injectionCast Natural (fun n: Natural => True) (n) _)). }
+    { smt_app IHm. smt_app (add_suc_r (injectionCast Natural (fun m: Natural => True) (n) _) (injectionCast Natural (fun n: Natural => True) (m) _)). }
 Qed.
 
 Definition add_assoc_spec: Prop. 
-Proof. now unshelve refine (forall (m:{m: Natural| True}) (n:{n: Natural| True}) (o:{o: Natural| True}), (` (add m (subsumptionCast Natural (fun VV: Natural => (` (add_unrefined m n))=VV) (fun n: Natural => True) _ (add n o))))=(` (add (subsumptionCast Natural (fun VV: Natural => (` (add_unrefined m n))=VV) (fun m: Natural => True) _ (add m n)) o))).
+Proof. now unshelve refine (forall (m:{m: Natural| True}) (n:{n: Natural| True}) (o:{o: Natural| True}), (` (add m (subsumptionCast Natural (fun VV: Natural => (` (add_unrefined m n))=VV) (fun n: Natural => True) _ (add n o))))=(` (add (subsumptionCast Natural (fun VV: Natural => (` (add_unrefined m n))=VV) (fun m: Natural => True) _ (add m n)) o))). .
 Defined.
 Theorem add_assoc: add_assoc_spec.
 Proof.
   intros m. intros n. intros o. destruct m as [m mp ].  destruct n as [n np ].  destruct o as [o op ]. 
-  induction m as [| m IHm ]. now smt_trivial. smt_app IHm.
+  induction m as [| m IHm ]. 
+    { now smt_trivial. }
+    { smt_app IHm. }
 Qed.
 
 Definition mult_suc_r_spec: Prop. 
-Proof. now unshelve refine (forall (n:{n: Natural| True}) (m:{m: Natural| True}), (` (mult n (injectionCast Natural (fun n: Natural => True) (fun n: Natural => I) (Suc (` (m))))))=(` (add n (subsumptionCast Natural (fun VV: Natural => (` (mult_unrefined m n))=VV) (fun n: Natural => True) _ (mult n m))))).
+Proof. now unshelve refine (forall (n:{n: Natural| True}) (m:{m: Natural| True}), (` (mult n (injectionCast Natural (fun n: Natural => True) (Suc (` (m))) _)))=(` (add n (subsumptionCast Natural (fun VV: Natural => (` (mult_unrefined m n))=VV) (fun n: Natural => True) _ (mult n m))))). .
 Defined.
 Theorem mult_suc_r: mult_suc_r_spec.
 Proof.
   intros n. intros m. destruct n as [n np ].  destruct m as [m mp ]. 
-  induction n as [| n IHn ]. now smt_trivial. smt_app IHn. smt_app (add_assoc (injectionCast Natural (fun m: Natural => True) (fun m: Natural => I) (m)) (injectionCast Natural (fun n: Natural => True) (fun n: Natural => I) (n)) (subsumptionCast Natural (fun VV: Natural => (` (mult_unrefined (injectionCast Natural (fun m: Natural => True) (fun m: Natural => I) (m)) (injectionCast Natural (fun n: Natural => True) (fun n: Natural => I) (n))))=VV) (fun o: Natural => True) _ (mult (injectionCast Natural (fun m: Natural => True) (fun m: Natural => I) (n)) (injectionCast Natural (fun n: Natural => True) (fun n: Natural => I) (m))))). smt_app (add_comm (injectionCast Natural (fun m: Natural => True) (fun m: Natural => I) (m)) (injectionCast Natural (fun n: Natural => True) (fun n: Natural => I) (n))). smt_app (add_assoc (injectionCast Natural (fun m: Natural => True) (fun m: Natural => I) (n)) (injectionCast Natural (fun n: Natural => True) (fun n: Natural => I) (m)) (subsumptionCast Natural (fun VV: Natural => (` (mult_unrefined (injectionCast Natural (fun m: Natural => True) (fun m: Natural => I) (m)) (injectionCast Natural (fun n: Natural => True) (fun n: Natural => I) (n))))=VV) (fun o: Natural => True) _ (mult (injectionCast Natural (fun m: Natural => True) (fun m: Natural => I) (n)) (injectionCast Natural (fun n: Natural => True) (fun n: Natural => I) (m))))).
+  induction n as [| n IHn ]. 
+    { now smt_trivial. }
+    { smt_app IHn. smt_app (add_assoc (injectionCast Natural (fun m: Natural => True) (m) _) (injectionCast Natural (fun n: Natural => True) (n) _) (subsumptionCast Natural (fun VV: Natural => (` (mult_unrefined (injectionCast Natural (fun m: Natural => True) (m) _) (injectionCast Natural (fun n: Natural => True) (n) _)))=VV) (fun o: Natural => True) _ (mult (injectionCast Natural (fun m: Natural => True) (n) _) (injectionCast Natural (fun n: Natural => True) (m) _)))). smt_app (add_comm (injectionCast Natural (fun m: Natural => True) (m) _) (injectionCast Natural (fun n: Natural => True) (n) _)). smt_app (add_assoc (injectionCast Natural (fun m: Natural => True) (n) _) (injectionCast Natural (fun n: Natural => True) (m) _) (subsumptionCast Natural (fun VV: Natural => (` (mult_unrefined (injectionCast Natural (fun m: Natural => True) (m) _) (injectionCast Natural (fun n: Natural => True) (n) _)))=VV) (fun o: Natural => True) _ (mult (injectionCast Natural (fun m: Natural => True) (n) _) (injectionCast Natural (fun n: Natural => True) (m) _)))). }
 Qed.
 
 Definition add_dist_rmult_spec: Prop. 
-Proof. now unshelve refine (forall (m:{m: Natural| True}) (n:{n: Natural| True}) (o:{o: Natural| True}), (` (mult (subsumptionCast Natural (fun VV: Natural => (` (add_unrefined m n))=VV) (fun m: Natural => True) _ (add m n)) o))=(` (add (subsumptionCast Natural (fun VV: Natural => (` (mult_unrefined m n))=VV) (fun m: Natural => True) _ (mult m o)) (subsumptionCast Natural (fun VV: Natural => (` (mult_unrefined m n))=VV) (fun n: Natural => True) _ (mult n o))))).
+Proof. now unshelve refine (forall (m:{m: Natural| True}) (n:{n: Natural| True}) (o:{o: Natural| True}), (` (mult (subsumptionCast Natural (fun VV: Natural => (` (add_unrefined m n))=VV) (fun m: Natural => True) _ (add m n)) o))=(` (add (subsumptionCast Natural (fun VV: Natural => (` (mult_unrefined m n))=VV) (fun m: Natural => True) _ (mult m o)) (subsumptionCast Natural (fun VV: Natural => (` (mult_unrefined m n))=VV) (fun n: Natural => True) _ (mult n o))))). .
 Defined.
 Theorem add_dist_rmult: add_dist_rmult_spec.
 Proof.
   intros m. intros n. intros o. destruct m as [m mp ].  destruct n as [n np ].  destruct o as [o op ]. 
-  induction m as [| m IHm ]. now smt_trivial. smt_app IHm. smt_app (add_assoc (injectionCast Natural (fun m: Natural => True) (fun m: Natural => I) (o)) (subsumptionCast Natural (fun VV: Natural => (` (mult_unrefined (injectionCast Natural (fun m: Natural => True) (fun m: Natural => I) (m)) (injectionCast Natural (fun n: Natural => True) (fun n: Natural => I) (n))))=VV) (fun n: Natural => True) _ (mult (injectionCast Natural (fun m: Natural => True) (fun m: Natural => I) (m)) (injectionCast Natural (fun n: Natural => True) (fun n: Natural => I) (o)))) (subsumptionCast Natural (fun VV: Natural => (` (mult_unrefined (injectionCast Natural (fun m: Natural => True) (fun m: Natural => I) (m)) (injectionCast Natural (fun n: Natural => True) (fun n: Natural => I) (n))))=VV) (fun o: Natural => True) _ (mult (injectionCast Natural (fun m: Natural => True) (fun m: Natural => I) (n)) (injectionCast Natural (fun n: Natural => True) (fun n: Natural => I) (o))))).
+  induction m as [| m IHm ]. 
+    { now smt_trivial. }
+    { smt_app IHm. smt_app (add_assoc (injectionCast Natural (fun m: Natural => True) (o) _) (subsumptionCast Natural (fun VV: Natural => (` (mult_unrefined (injectionCast Natural (fun m: Natural => True) (m) _) (injectionCast Natural (fun n: Natural => True) (n) _)))=VV) (fun n: Natural => True) _ (mult (injectionCast Natural (fun m: Natural => True) (m) _) (injectionCast Natural (fun n: Natural => True) (o) _))) (subsumptionCast Natural (fun VV: Natural => (` (mult_unrefined (injectionCast Natural (fun m: Natural => True) (m) _) (injectionCast Natural (fun n: Natural => True) (n) _)))=VV) (fun o: Natural => True) _ (mult (injectionCast Natural (fun m: Natural => True) (n) _) (injectionCast Natural (fun n: Natural => True) (o) _)))). }
 Qed.
 
 Definition mult_assoc_spec: Prop. 
-Proof. now unshelve refine (forall (m:{m: Natural| True}) (n:{n: Natural| True}) (o:{o: Natural| True}), (` (mult (subsumptionCast Natural (fun VV: Natural => (` (mult_unrefined m n))=VV) (fun m: Natural => True) _ (mult m n)) o))=(` (mult m (subsumptionCast Natural (fun VV: Natural => (` (mult_unrefined m n))=VV) (fun n: Natural => True) _ (mult n o))))).
+Proof. now unshelve refine (forall (m:{m: Natural| True}) (n:{n: Natural| True}) (o:{o: Natural| True}), (` (mult (subsumptionCast Natural (fun VV: Natural => (` (mult_unrefined m n))=VV) (fun m: Natural => True) _ (mult m n)) o))=(` (mult m (subsumptionCast Natural (fun VV: Natural => (` (mult_unrefined m n))=VV) (fun n: Natural => True) _ (mult n o))))). .
 Defined.
 Theorem mult_assoc: mult_assoc_spec.
 Proof.
   intros m. intros n. intros o. destruct m as [m mp ].  destruct n as [n np ].  destruct o as [o op ]. 
-  induction m as [| m IHm ]. now smt_trivial. 
-  assertFresh ((` (mult (subsumptionCast Natural (fun VV: Natural => (` (mult_unrefined (injectionCast Natural (fun m: Natural => True) (fun m: Natural => I) (m)) (injectionCast Natural (fun n: Natural => True) (fun n: Natural => I) (n))))=VV) (fun m: Natural => True) _ (mult (injectionCast Natural (fun m: Natural => True) (fun m: Natural => I) (Suc m)) (injectionCast Natural (fun n: Natural => True) (fun n: Natural => I) (n)))) (injectionCast Natural (fun n: Natural => True) (fun n: Natural => I) (o))))=(` (mult (subsumptionCast Natural (fun VV: Natural => (` (add_unrefined (injectionCast Natural (fun m: Natural => True) (fun m: Natural => I) (m)) (injectionCast Natural (fun n: Natural => True) (fun n: Natural => I) (n))))=VV) (fun m: Natural => True) _ (add (injectionCast Natural (fun m: Natural => True) (fun m: Natural => I) (n)) (subsumptionCast Natural (fun VV: Natural => (` (mult_unrefined (injectionCast Natural (fun m: Natural => True) (fun m: Natural => I) (m)) (injectionCast Natural (fun n: Natural => True) (fun n: Natural => I) (n))))=VV) (fun n: Natural => True) _ (mult (injectionCast Natural (fun m: Natural => True) (fun m: Natural => I) (m)) (injectionCast Natural (fun n: Natural => True) (fun n: Natural => I) (n)))))) (injectionCast Natural (fun n: Natural => True) (fun n: Natural => I) (o))))) as lem using smt_trivial. 
-  assertFresh ((` (mult (subsumptionCast Natural (fun VV: Natural => (` (add_unrefined (injectionCast Natural (fun m: Natural => True) (fun m: Natural => I) (m)) (injectionCast Natural (fun n: Natural => True) (fun n: Natural => I) (n))))=VV) (fun m: Natural => True) _ (add (injectionCast Natural (fun m: Natural => True) (fun m: Natural => I) (n)) (subsumptionCast Natural (fun VV: Natural => (` (mult_unrefined (injectionCast Natural (fun m: Natural => True) (fun m: Natural => I) (m)) (injectionCast Natural (fun n: Natural => True) (fun n: Natural => I) (n))))=VV) (fun n: Natural => True) _ (mult (injectionCast Natural (fun m: Natural => True) (fun m: Natural => I) (m)) (injectionCast Natural (fun n: Natural => True) (fun n: Natural => I) (n)))))) (injectionCast Natural (fun n: Natural => True) (fun n: Natural => I) (o))))=(` (add (subsumptionCast Natural (fun VV: Natural => (` (mult_unrefined (injectionCast Natural (fun m: Natural => True) (fun m: Natural => I) (m)) (injectionCast Natural (fun n: Natural => True) (fun n: Natural => I) (n))))=VV) (fun m: Natural => True) _ (mult (injectionCast Natural (fun m: Natural => True) (fun m: Natural => I) (n)) (injectionCast Natural (fun n: Natural => True) (fun n: Natural => I) (o)))) (subsumptionCast Natural (fun VV: Natural => (` (mult_unrefined (injectionCast Natural (fun m: Natural => True) (fun m: Natural => I) (m)) (injectionCast Natural (fun n: Natural => True) (fun n: Natural => I) (n))))=VV) (fun n: Natural => True) _ (mult (subsumptionCast Natural (fun VV: Natural => (` (mult_unrefined (injectionCast Natural (fun m: Natural => True) (fun m: Natural => I) (m)) (injectionCast Natural (fun n: Natural => True) (fun n: Natural => I) (n))))=VV) (fun m: Natural => True) _ (mult (injectionCast Natural (fun m: Natural => True) (fun m: Natural => I) (m)) (injectionCast Natural (fun n: Natural => True) (fun n: Natural => I) (n)))) (injectionCast Natural (fun n: Natural => True) (fun n: Natural => I) (o))))))) as lem using (smt_app (add_dist_rmult (injectionCast Natural (fun m: Natural => True) (fun m: Natural => I) (n)) (subsumptionCast Natural (fun VV: Natural => (` (mult_unrefined (injectionCast Natural (fun m: Natural => True) (fun m: Natural => I) (m)) (injectionCast Natural (fun n: Natural => True) (fun n: Natural => I) (n))))=VV) (fun n: Natural => True) _ (mult (injectionCast Natural (fun m: Natural => True) (fun m: Natural => I) (m)) (injectionCast Natural (fun n: Natural => True) (fun n: Natural => I) (n)))) (injectionCast Natural (fun o: Natural => True) (fun o: Natural => I) (o)))). 
-  assertFresh ((` (add (subsumptionCast Natural (fun VV: Natural => (` (mult_unrefined (injectionCast Natural (fun m: Natural => True) (fun m: Natural => I) (m)) (injectionCast Natural (fun n: Natural => True) (fun n: Natural => I) (n))))=VV) (fun m: Natural => True) _ (mult (injectionCast Natural (fun m: Natural => True) (fun m: Natural => I) (n)) (injectionCast Natural (fun n: Natural => True) (fun n: Natural => I) (o)))) (subsumptionCast Natural (fun VV: Natural => (` (mult_unrefined (injectionCast Natural (fun m: Natural => True) (fun m: Natural => I) (m)) (injectionCast Natural (fun n: Natural => True) (fun n: Natural => I) (n))))=VV) (fun n: Natural => True) _ (mult (subsumptionCast Natural (fun VV: Natural => (` (mult_unrefined (injectionCast Natural (fun m: Natural => True) (fun m: Natural => I) (m)) (injectionCast Natural (fun n: Natural => True) (fun n: Natural => I) (n))))=VV) (fun m: Natural => True) _ (mult (injectionCast Natural (fun m: Natural => True) (fun m: Natural => I) (m)) (injectionCast Natural (fun n: Natural => True) (fun n: Natural => I) (n)))) (injectionCast Natural (fun n: Natural => True) (fun n: Natural => I) (o))))))=(` (add (subsumptionCast Natural (fun VV: Natural => (` (mult_unrefined (injectionCast Natural (fun m: Natural => True) (fun m: Natural => I) (m)) (injectionCast Natural (fun n: Natural => True) (fun n: Natural => I) (n))))=VV) (fun m: Natural => True) _ (mult (injectionCast Natural (fun m: Natural => True) (fun m: Natural => I) (n)) (injectionCast Natural (fun n: Natural => True) (fun n: Natural => I) (o)))) (subsumptionCast Natural (fun VV: Natural => (` (mult_unrefined (injectionCast Natural (fun m: Natural => True) (fun m: Natural => I) (m)) (injectionCast Natural (fun n: Natural => True) (fun n: Natural => I) (n))))=VV) (fun n: Natural => True) _ (mult (injectionCast Natural (fun m: Natural => True) (fun m: Natural => I) (m)) (subsumptionCast Natural (fun VV: Natural => (` (mult_unrefined (injectionCast Natural (fun m: Natural => True) (fun m: Natural => I) (m)) (injectionCast Natural (fun n: Natural => True) (fun n: Natural => I) (n))))=VV) (fun n: Natural => True) _ (mult (injectionCast Natural (fun m: Natural => True) (fun m: Natural => I) (n)) (injectionCast Natural (fun n: Natural => True) (fun n: Natural => I) (o))))))))) as lem using (smt_app IHm). now 
-  assertFresh ((` (add (subsumptionCast Natural (fun VV: Natural => (` (mult_unrefined (injectionCast Natural (fun m: Natural => True) (fun m: Natural => I) (m)) (injectionCast Natural (fun n: Natural => True) (fun n: Natural => I) (n))))=VV) (fun m: Natural => True) _ (mult (injectionCast Natural (fun m: Natural => True) (fun m: Natural => I) (n)) (injectionCast Natural (fun n: Natural => True) (fun n: Natural => I) (o)))) (subsumptionCast Natural (fun VV: Natural => (` (mult_unrefined (injectionCast Natural (fun m: Natural => True) (fun m: Natural => I) (m)) (injectionCast Natural (fun n: Natural => True) (fun n: Natural => I) (n))))=VV) (fun n: Natural => True) _ (mult (injectionCast Natural (fun m: Natural => True) (fun m: Natural => I) (m)) (subsumptionCast Natural (fun VV: Natural => (` (mult_unrefined (injectionCast Natural (fun m: Natural => True) (fun m: Natural => I) (m)) (injectionCast Natural (fun n: Natural => True) (fun n: Natural => I) (n))))=VV) (fun n: Natural => True) _ (mult (injectionCast Natural (fun m: Natural => True) (fun m: Natural => I) (n)) (injectionCast Natural (fun n: Natural => True) (fun n: Natural => I) (o))))))))=(` (mult (injectionCast Natural (fun m: Natural => True) (fun m: Natural => I) (Suc m)) (subsumptionCast Natural (fun VV: Natural => (` (mult_unrefined (injectionCast Natural (fun m: Natural => True) (fun m: Natural => I) (m)) (injectionCast Natural (fun n: Natural => True) (fun n: Natural => I) (n))))=VV) (fun n: Natural => True) _ (mult (injectionCast Natural (fun m: Natural => True) (fun m: Natural => I) (n)) (injectionCast Natural (fun n: Natural => True) (fun n: Natural => I) (o))))))) as lem using smt_trivial.
+  induction m as [| m IHm ]. 
+    { now smt_trivial. }
+    { 
+  assertFresh ((` (mult (subsumptionCast Natural (fun VV: Natural => (` (mult_unrefined (injectionCast Natural (fun m: Natural => True) (m) _) (injectionCast Natural (fun n: Natural => True) (n) _)))=VV) (fun m: Natural => True) _ (mult (injectionCast Natural (fun m: Natural => True) (Suc m) _) (injectionCast Natural (fun n: Natural => True) (n) _))) (injectionCast Natural (fun n: Natural => True) (o) _)))=(` (mult (subsumptionCast Natural (fun VV: Natural => (` (add_unrefined (injectionCast Natural (fun m: Natural => True) (m) _) (injectionCast Natural (fun n: Natural => True) (n) _)))=VV) (fun m: Natural => True) _ (add (injectionCast Natural (fun m: Natural => True) (n) _) (subsumptionCast Natural (fun VV: Natural => (` (mult_unrefined (injectionCast Natural (fun m: Natural => True) (m) _) (injectionCast Natural (fun n: Natural => True) (n) _)))=VV) (fun n: Natural => True) _ (mult (injectionCast Natural (fun m: Natural => True) (m) _) (injectionCast Natural (fun n: Natural => True) (n) _))))) (injectionCast Natural (fun n: Natural => True) (o) _)))) as lem using smt_trivial. . 
+  assertFresh ((` (mult (subsumptionCast Natural (fun VV: Natural => (` (add_unrefined (injectionCast Natural (fun m: Natural => True) (m) _) (injectionCast Natural (fun n: Natural => True) (n) _)))=VV) (fun m: Natural => True) _ (add (injectionCast Natural (fun m: Natural => True) (n) _) (subsumptionCast Natural (fun VV: Natural => (` (mult_unrefined (injectionCast Natural (fun m: Natural => True) (m) _) (injectionCast Natural (fun n: Natural => True) (n) _)))=VV) (fun n: Natural => True) _ (mult (injectionCast Natural (fun m: Natural => True) (m) _) (injectionCast Natural (fun n: Natural => True) (n) _))))) (injectionCast Natural (fun n: Natural => True) (o) _)))=(` (add (subsumptionCast Natural (fun VV: Natural => (` (mult_unrefined (injectionCast Natural (fun m: Natural => True) (m) _) (injectionCast Natural (fun n: Natural => True) (n) _)))=VV) (fun m: Natural => True) _ (mult (injectionCast Natural (fun m: Natural => True) (n) _) (injectionCast Natural (fun n: Natural => True) (o) _))) (subsumptionCast Natural (fun VV: Natural => (` (mult_unrefined (injectionCast Natural (fun m: Natural => True) (m) _) (injectionCast Natural (fun n: Natural => True) (n) _)))=VV) (fun n: Natural => True) _ (mult (subsumptionCast Natural (fun VV: Natural => (` (mult_unrefined (injectionCast Natural (fun m: Natural => True) (m) _) (injectionCast Natural (fun n: Natural => True) (n) _)))=VV) (fun m: Natural => True) _ (mult (injectionCast Natural (fun m: Natural => True) (m) _) (injectionCast Natural (fun n: Natural => True) (n) _))) (injectionCast Natural (fun n: Natural => True) (o) _)))))) as lem using (smt_app (add_dist_rmult (injectionCast Natural (fun m: Natural => True) (n) _) (subsumptionCast Natural (fun VV: Natural => (` (mult_unrefined (injectionCast Natural (fun m: Natural => True) (m) _) (injectionCast Natural (fun n: Natural => True) (n) _)))=VV) (fun n: Natural => True) _ (mult (injectionCast Natural (fun m: Natural => True) (m) _) (injectionCast Natural (fun n: Natural => True) (n) _))) (injectionCast Natural (fun o: Natural => True) (o) _)). ). 
+  assertFresh ((` (add (subsumptionCast Natural (fun VV: Natural => (` (mult_unrefined (injectionCast Natural (fun m: Natural => True) (m) _) (injectionCast Natural (fun n: Natural => True) (n) _)))=VV) (fun m: Natural => True) _ (mult (injectionCast Natural (fun m: Natural => True) (n) _) (injectionCast Natural (fun n: Natural => True) (o) _))) (subsumptionCast Natural (fun VV: Natural => (` (mult_unrefined (injectionCast Natural (fun m: Natural => True) (m) _) (injectionCast Natural (fun n: Natural => True) (n) _)))=VV) (fun n: Natural => True) _ (mult (subsumptionCast Natural (fun VV: Natural => (` (mult_unrefined (injectionCast Natural (fun m: Natural => True) (m) _) (injectionCast Natural (fun n: Natural => True) (n) _)))=VV) (fun m: Natural => True) _ (mult (injectionCast Natural (fun m: Natural => True) (m) _) (injectionCast Natural (fun n: Natural => True) (n) _))) (injectionCast Natural (fun n: Natural => True) (o) _)))))=(` (add (subsumptionCast Natural (fun VV: Natural => (` (mult_unrefined (injectionCast Natural (fun m: Natural => True) (m) _) (injectionCast Natural (fun n: Natural => True) (n) _)))=VV) (fun m: Natural => True) _ (mult (injectionCast Natural (fun m: Natural => True) (n) _) (injectionCast Natural (fun n: Natural => True) (o) _))) (subsumptionCast Natural (fun VV: Natural => (` (mult_unrefined (injectionCast Natural (fun m: Natural => True) (m) _) (injectionCast Natural (fun n: Natural => True) (n) _)))=VV) (fun n: Natural => True) _ (mult (injectionCast Natural (fun m: Natural => True) (m) _) (subsumptionCast Natural (fun VV: Natural => (` (mult_unrefined (injectionCast Natural (fun m: Natural => True) (m) _) (injectionCast Natural (fun n: Natural => True) (n) _)))=VV) (fun n: Natural => True) _ (mult (injectionCast Natural (fun m: Natural => True) (n) _) (injectionCast Natural (fun n: Natural => True) (o) _)))))))) as lem using (smt_app IHm. ). now 
+  assertFresh ((` (add (subsumptionCast Natural (fun VV: Natural => (` (mult_unrefined (injectionCast Natural (fun m: Natural => True) (m) _) (injectionCast Natural (fun n: Natural => True) (n) _)))=VV) (fun m: Natural => True) _ (mult (injectionCast Natural (fun m: Natural => True) (n) _) (injectionCast Natural (fun n: Natural => True) (o) _))) (subsumptionCast Natural (fun VV: Natural => (` (mult_unrefined (injectionCast Natural (fun m: Natural => True) (m) _) (injectionCast Natural (fun n: Natural => True) (n) _)))=VV) (fun n: Natural => True) _ (mult (injectionCast Natural (fun m: Natural => True) (m) _) (subsumptionCast Natural (fun VV: Natural => (` (mult_unrefined (injectionCast Natural (fun m: Natural => True) (m) _) (injectionCast Natural (fun n: Natural => True) (n) _)))=VV) (fun n: Natural => True) _ (mult (injectionCast Natural (fun m: Natural => True) (n) _) (injectionCast Natural (fun n: Natural => True) (o) _)))))))=(` (mult (injectionCast Natural (fun m: Natural => True) (Suc m) _) (subsumptionCast Natural (fun VV: Natural => (` (mult_unrefined (injectionCast Natural (fun m: Natural => True) (m) _) (injectionCast Natural (fun n: Natural => True) (n) _)))=VV) (fun n: Natural => True) _ (mult (injectionCast Natural (fun m: Natural => True) (n) _) (injectionCast Natural (fun n: Natural => True) (o) _)))))) as lem using smt_trivial. . }
 Qed.
 
 Definition mult_zero_l_spec: Prop. 
-Proof. now unshelve refine (forall (n:{n: Natural| True}), (` (mult (injectionCast Natural (fun m: Natural => True) (fun m: Natural => I) (ZeroN)) n))=ZeroN).
+Proof. now unshelve refine (forall (n:{n: Natural| True}), (` (mult (injectionCast Natural (fun m: Natural => True) (ZeroN) _) n))=ZeroN). .
 Defined.
 Theorem mult_zero_l: mult_zero_l_spec.
 Proof.
   intros n. destruct n as [n np ]. 
-  induction n as [| n IHn ]. now smt_trivial. smt_app IHn.
+  induction n as [| n IHn ]. 
+    { now smt_trivial. }
+    { smt_app IHn. }
 Qed.
 
 Definition mult_suc_l_spec: Prop. 
-Proof. now unshelve refine (forall (m:{m: Natural| True}) (n:{n: Natural| True}), (` (mult (injectionCast Natural (fun m: Natural => True) (fun m: Natural => I) (Suc (` (m)))) n))=(` (add n (subsumptionCast Natural (fun VV: Natural => (` (mult_unrefined m n))=VV) (fun n: Natural => True) _ (mult m n))))).
+Proof. now unshelve refine (forall (m:{m: Natural| True}) (n:{n: Natural| True}), (` (mult (injectionCast Natural (fun m: Natural => True) (Suc (` (m))) _) n))=(` (add n (subsumptionCast Natural (fun VV: Natural => (` (mult_unrefined m n))=VV) (fun n: Natural => True) _ (mult m n))))). .
 Defined.
 Theorem mult_suc_l: mult_suc_l_spec.
 Proof.
   intros m. intros n. destruct m as [m mp ].  destruct n as [n np ]. 
-  destruct m as [ | m ]. now smt_trivial. now smt_trivial.
+  
+    { destruct m as [ | m ]. now smt_trivial. now smt_trivial. }
 Qed.
 
 Definition mult_zero_r_spec: Prop. 
-Proof. now unshelve refine (forall (n:{n: Natural| True}), (` (mult n (injectionCast Natural (fun n: Natural => True) (fun n: Natural => I) (ZeroN))))=ZeroN).
+Proof. now unshelve refine (forall (n:{n: Natural| True}), (` (mult n (injectionCast Natural (fun n: Natural => True) (ZeroN) _)))=ZeroN). .
 Defined.
 Theorem mult_zero_r: mult_zero_r_spec.
 Proof.
   intros n. destruct n as [n np ]. 
-  induction n as [| n IHn ]. now smt_trivial. smt_app IHn.
+  induction n as [| n IHn ]. 
+    { now smt_trivial. }
+    { smt_app IHn. }
 Qed.
 
 Definition add_dist_lmult_spec: Prop. 
-Proof. now unshelve refine (forall (m:{m: Natural| True}) (n:{n: Natural| True}) (o:{o: Natural| True}), (` (mult m (subsumptionCast Natural (fun VV: Natural => (` (add_unrefined m n))=VV) (fun n: Natural => True) _ (add n o))))=(` (add (subsumptionCast Natural (fun VV: Natural => (` (mult_unrefined m n))=VV) (fun m: Natural => True) _ (mult m n)) (subsumptionCast Natural (fun VV: Natural => (` (mult_unrefined m n))=VV) (fun n: Natural => True) _ (mult m o))))).
+Proof. now unshelve refine (forall (m:{m: Natural| True}) (n:{n: Natural| True}) (o:{o: Natural| True}), (` (mult m (subsumptionCast Natural (fun VV: Natural => (` (add_unrefined m n))=VV) (fun n: Natural => True) _ (add n o))))=(` (add (subsumptionCast Natural (fun VV: Natural => (` (mult_unrefined m n))=VV) (fun m: Natural => True) _ (mult m n)) (subsumptionCast Natural (fun VV: Natural => (` (mult_unrefined m n))=VV) (fun n: Natural => True) _ (mult m o))))). .
 Defined.
 Theorem add_dist_lmult: add_dist_lmult_spec.
 Proof.
   intros m. intros n. intros o. destruct m as [m mp ].  destruct n as [n np ].  destruct o as [o op ]. 
-  induction n as [| n IHn ]. smt_app (mult_zero_r (injectionCast Natural (fun n: Natural => True) (fun n: Natural => I) (m))). smt_app (mult_suc_r (injectionCast Natural (fun n: Natural => True) (fun n: Natural => I) (m)) (subsumptionCast Natural (fun VV: Natural => (` (add_unrefined (injectionCast Natural (fun m: Natural => True) (fun m: Natural => I) (m)) (injectionCast Natural (fun n: Natural => True) (fun n: Natural => I) (n))))=VV) (fun m: Natural => True) _ (add (injectionCast Natural (fun m: Natural => True) (fun m: Natural => I) (n)) (injectionCast Natural (fun n: Natural => True) (fun n: Natural => I) (o))))). smt_app IHn. smt_app (add_assoc (injectionCast Natural (fun m: Natural => True) (fun m: Natural => I) (m)) (subsumptionCast Natural (fun VV: Natural => (` (mult_unrefined (injectionCast Natural (fun m: Natural => True) (fun m: Natural => I) (m)) (injectionCast Natural (fun n: Natural => True) (fun n: Natural => I) (n))))=VV) (fun n: Natural => True) _ (mult (injectionCast Natural (fun m: Natural => True) (fun m: Natural => I) (m)) (injectionCast Natural (fun n: Natural => True) (fun n: Natural => I) (n)))) (subsumptionCast Natural (fun VV: Natural => (` (mult_unrefined (injectionCast Natural (fun m: Natural => True) (fun m: Natural => I) (m)) (injectionCast Natural (fun n: Natural => True) (fun n: Natural => I) (n))))=VV) (fun o: Natural => True) _ (mult (injectionCast Natural (fun m: Natural => True) (fun m: Natural => I) (m)) (injectionCast Natural (fun n: Natural => True) (fun n: Natural => I) (o))))). smt_app (mult_suc_r (injectionCast Natural (fun n: Natural => True) (fun n: Natural => I) (m)) (injectionCast Natural (fun m: Natural => True) (fun m: Natural => I) (n))).
+  induction n as [| n IHn ]. 
+    { smt_app (mult_zero_r (injectionCast Natural (fun n: Natural => True) (m) _)). }
+    { smt_app (mult_suc_r (injectionCast Natural (fun n: Natural => True) (m) _) (subsumptionCast Natural (fun VV: Natural => (` (add_unrefined (injectionCast Natural (fun m: Natural => True) (m) _) (injectionCast Natural (fun n: Natural => True) (n) _)))=VV) (fun m: Natural => True) _ (add (injectionCast Natural (fun m: Natural => True) (n) _) (injectionCast Natural (fun n: Natural => True) (o) _)))). smt_app IHn. smt_app (add_assoc (injectionCast Natural (fun m: Natural => True) (m) _) (subsumptionCast Natural (fun VV: Natural => (` (mult_unrefined (injectionCast Natural (fun m: Natural => True) (m) _) (injectionCast Natural (fun n: Natural => True) (n) _)))=VV) (fun n: Natural => True) _ (mult (injectionCast Natural (fun m: Natural => True) (m) _) (injectionCast Natural (fun n: Natural => True) (n) _))) (subsumptionCast Natural (fun VV: Natural => (` (mult_unrefined (injectionCast Natural (fun m: Natural => True) (m) _) (injectionCast Natural (fun n: Natural => True) (n) _)))=VV) (fun o: Natural => True) _ (mult (injectionCast Natural (fun m: Natural => True) (m) _) (injectionCast Natural (fun n: Natural => True) (o) _)))). smt_app (mult_suc_r (injectionCast Natural (fun n: Natural => True) (m) _) (injectionCast Natural (fun m: Natural => True) (n) _)). }
 Qed.
 
 Definition mult_one_r_spec: Prop. 
-Proof. now unshelve refine (forall (n:{n: Natural| True}), (` (mult n (injectionCast Natural (fun n: Natural => True) (fun n: Natural => I) (one))))=(` (n))).
+Proof. now unshelve refine (forall (n:{n: Natural| True}), (` (mult n (injectionCast Natural (fun n: Natural => True) (one) _)))=(` (n))). .
 Defined.
 Theorem mult_one_r: mult_one_r_spec.
 Proof.
   intros n. destruct n as [n np ]. 
-  induction n as [| n IHn ]. now smt_trivial. smt_app IHn.
+  induction n as [| n IHn ]. 
+    { now smt_trivial. }
+    { smt_app IHn. }
 Qed.
